Test/HeapLangExamples.lean
@@ -7,11 +7,21 @@ open ITree.Exec
 namespace HeapLang
 
 example s :
-  exec heaplangEH (Exp.denote (.binop .plus (.val 1) (.val 1))) s λ t _ => t = return (.lit $ .int 2) := by
+  exec heaplangEH hl(#1 + #1).denote s λ t _ => t = return (.lit $ .int 2) := by
     simp [Exp.denote, Exp.isVal, BinOp.denote, BinOp.evalInt]
-    -- apply exec.bind
-    -- simp [Val.int!]
-    -- apply exec.stop
-    -- simp
+    apply exec.stop
+    simp
+
+example tid tpool heap :
+  tid < tpool.length →
+  exec heaplangEH hl(let x := #1; x + #1).denote ⟨tid, tpool, heap⟩ λ t _ => t = return (.lit $ .int 2) := by
+    intro _
+    simp [Exp.denote, Exp.isVal, Exp.subst, Exp.substStr, yieldAfter, Exp.yieldIfNotVal, Val.rec!, BinOp.denote, BinOp.evalInt, -bind_pure_comp]
+    apply exec_yield_same
+    · simp [*]
+    simp [-bind_pure_comp]
+    apply exec_yield_same
+    · simp [*]
+    simp [-bind_pure_comp]
     apply exec.stop
     simp
